\documentclass[CheatSheet]{subfiles}
\begin{document}
\summarystyle

\section{Gauge theory}
\paragraph{SU(2)}
Fundamental representation $\TWO=(T^a)_{ij}$,
adjoint representation $\text{adj.}=(\epsilon^{a})^{bc}$.%
\footnote{We do not distinguish sub- and superscripts for gauge indices.}
\begin{align*}
 T_a &= \frac{1}{2} \sigma_a,
&
 \Tr(T_a T_b) &= \frac{1}{2}\delta_{ab},
&
 [T_a, T_b] &= \ii \epsilon^{abc}T^c,
&
 \epsilon^{abc}\epsilon^{ade} &= \delta_{bd}\delta_{ce} - \delta_{be}\delta_{cd}
\end{align*}
Since
$\overline{\TWO}
  = -(T^a)^*_{ij}$
has identities
 $-\epsilon T^a \epsilon = -T^{a*}$ and
 $-\epsilon (-T^{a*}) \epsilon = T^a$,
%
%\begin{equation}
% $-\epsilon T^a \epsilon = -T^{a*}$,
%\end{equation}
%  = -\epsilon^{ik}T^a_{kl}\epsilon^{lj}
%  = (\epsilon T^a\epsilon^{-1})_{ij}
we see that $\epsilon^{ab}\TWO^b$ transforms as $\overline{\TWO}^a$:
\begin{equation}
 \epsilon^{ab}\TWO^b
\to
 \epsilon^{ab}[\exp\left(\ii g \theta^\alpha T^\alpha\right)]^{bc}\TWO^{c}
=
 \epsilon^{ab}[\exp\left(\ii g \theta^\alpha T^\alpha\right)]^{bc}(\epsilon^{-1})^{cd}(\epsilon^{de}\TWO^e)
=
 [\exp\left(-\ii g \theta^\alpha T^{\alpha*}\right)]^{ab}(\epsilon^{bc}\TWO^c).
\end{equation}

\paragraph{SU(3)}
Fundamental representation $\THREE=(\tau^a)_{ij}$,
$\THREEbar=-(\tau^{a})^*_{ij}$;
adjoint representation $\text{adj.}=\boldsymbol{8}=(f^{a})^{bc}$.%

Gell-Mann matrices:
\begin{align}
 \lambda_{1\text{--}8} &=
  \left(\begin{smallmatrix} 0&1&0 \\ 1&0&0 \\ 0&0&0 \end{smallmatrix}\right),
  \left(\begin{smallmatrix} 0&-\ii&0 \\ \ii&0&0 \\ 0&0&0  \end{smallmatrix}\right),
  \left(\begin{smallmatrix} 1&0&0 \\ 0&-1&0 \\ 0&0&0  \end{smallmatrix}\right),
  \left(\begin{smallmatrix} 0&0&1 \\ 0&0&0 \\ 1&0&0  \end{smallmatrix}\right),
  \left(\begin{smallmatrix} 0&0&-\ii \\ 0&0&0 \\ \ii&0&0  \end{smallmatrix}\right),
  \left(\begin{smallmatrix} 0&0&0 \\ 0&0&1 \\ 0&1&0  \end{smallmatrix}\right),
  \left(\begin{smallmatrix} 0&0&0 \\ 0&0&-\ii \\ 0&\ii&0  \end{smallmatrix}\right),
  \tfrac1{\sqrt3}\left(\begin{smallmatrix} 1&0&0 \\ 0&1&0 \\ 0&0&-2 \end{smallmatrix}\right).
\end{align}

\begin{align*}
 \tau_a &= \frac{1}{2} \lambda_a,
&
 \Tr(\tau_a \tau_b) &= \frac{1}{2}\delta_{ab},
&
 [\tau_a, \tau_b] &= \ii f^{abc}\tau^c,
&
 f^{ade}f^{bcd} + f^{bde}f^{cad} + f^{cde}f^{abd} &= 0.
\end{align*}

\begin{align*}
\THREE:~~\phi_a&
  \to [\exp(\ii g \theta^\alpha \tau^\alpha)]_{ab}\phi_b
  \simeq \phi_a + \ii g \theta^\alpha \tau^\alpha_{ab}\phi_b
&
\THREEbar:~~\phi_a&
  \to[\exp(-\ii g \theta^\alpha \tau^{\alpha*})]_{ab}\phi_b
  \simeq \phi_a - \ii g \theta^\alpha \tau^{\alpha*}_{ab}\phi_b
\\
\phi_a^*&
  \to[\exp(-\ii g \theta^\alpha \tau^{\alpha*})]_{ab}\phi_b^*
 \simeq \phi_a^* - \ii g \theta^\alpha \tau^{\alpha*}_{ab}\phi_b^*
&
\phi_a^*&
  \to[\exp(\ii g \theta^\alpha \tau^{\alpha})]_{ab}\phi_b^*
  \simeq \phi_a^* + \ii g \theta^\alpha \tau^{\alpha}_{ab}\phi_b^*
\\
&=\phi_b^*[\exp(-\ii g \theta^\alpha \tau^{\alpha})]_{ba}
 \simeq \phi_a^* - \ii g \theta^\alpha \phi_b^* \tau^{\alpha}_{ba}
\end{align*}
\end{document}
