%#!latexmk CheatSheet.tex
%%% Time-Stamp: <2009-07-05 14:08:17>
\section{General Definitions and Tools}
\subsection{Notations and Conventions}
\subsubsection{Metric etc.}

\begin{tabular}{l@{ :\ \ \ }l}
Minkowski Metric   & $\Hmn = \diag(+,-,-,-)$\\
Coordinates        & $\displaystyle x^\mu = (t,x,y,z)$; \quad Therefore $\Pm = \left(\pbib{}t,\vgrad\right)$\\
Gamma Matrices     & $\{\Gm,\Gn\}=2\Hmn;\quad \G5=\ii\G0\G1\G2\G3$\\[1zw]
Gamma Combinations & $1, \{\Gm\}, \{\sigma^{\mu\nu}\}, \{\Gm\G5\}, \G5;\quad
                      \sigma^{\mu\nu}=\frac\ii2[\Gm,\Gn]=0\Big/\ii\Gm\Gn$\\
\end{tabular}

\subsubsection{Fields}
\begin{tabular}{l@{ :\ \ \ }l}
Klein-Gordon Equation & $|\Pm \phi|^2-m^2|\phi|^2=0$\\
Klein-Gordon Field    &
    $\displaystyle\phi(x)=\intP3 \frac{1}{\sqrt{2E_{\vc p}}}
            \Bigl[a_\vc p\ee^{-\ii px} + b^\dagger_\vc p \ee^{\ii px}\Bigr]$\\[1.5zw]
Dirac Equation   & $(i\slashed\partial-m)\psi(x)=0$\\
Dirac Field      &
    $\displaystyle\psi(x)=\intP3 \frac{1}{\sqrt{2E_{\vc p}}}
     \sum_{s=1,2}\Bigl[a^s_\vc p u^s(p)\ee^{-\ii px}
                     + b^{s\dagger}_\vc p v^s(p)\ee^{\ii px}\Bigr]$\\[1.5zw]
Gauge Boson & $(\Psq+m^2)A^\mu(x)=0$\quad \text{\footnotesize (Real Klein-Gordon Equation)}\\
\quad{\footnotesize(Before Gauge Fixing)}
  & $\displaystyle A^\mu(x)=\intP3 \frac{1}{\sqrt{2E_{\vc p}}}
     \sum_{r=0,1,2,3}\Bigl[a^r_\vc p \epsilon^r(p)\ee^{-\ii px}
                     + a^{r\dagger}_\vc p \epsilon^{r*}(p)\ee^{\ii px}\Bigr]$\\[1.5zw]
ìÏïî-Goldstone Boson & \TODO.
\end{tabular}
\begin{rightnote}
\Subparagraph{Chiral Notation}
\begin{tabular}{l@{ :\ \ \ }l}
Gamma Matrices & $\Gm=\pmat{0&\Sm\\\bSm&0};\quad \G5=\pmat{-1&0\\0&1}$\\
Dirac Field    & $\psi    =\pmat{\psi\s L\\\psi\s R}; \quad
                  \bar\psi=\psi^\dagger\G0=\pmat{\psi\s R^\dagger&\psi\s L^\dagger}$\\
 & $u^s(p)=\pmat{\sqrt{p\cdot\sigma}\xi^s\\\sqrt{p\cdot\bar\sigma}\xi^s};\quad
    v^s(p)=\pmat{\sqrt{p\cdot\sigma}\eta^s\\-\sqrt{p\cdot\bar\sigma}\eta^s}$
  $\Bigl[\eta^s=\xi^{-s}:=-\ii\sigma^2(\xi^s)^*=(\xi^2,-\xi^1)\Bigr]$\\

Weyl Equations & $\ii\bar\sigma\cdot\partial\psi_L=m\psi_R;\quad
                  \ii\sigma\cdot\partial\psi_L=m\psi_L$\\


CPT transf.
 & $P\psi(t,\vc x) P = \eta\G0\psi(t,-\vc x)\quad(|\eta|^2=1)$\\
 & $T\psi(t,\vc x) T = \G1\G3\psi(-t,\vc x)\quad\text{(ignoring intrinsic phase)}$\\
 & $C\psi(t,\vc x) C = -\ii\G2\psi^*(t,\vc x) = -\ii\trans{(\bar\psi\G0\G2)}\quad
                       \text{(ÅV)}$\\
 & $\bar\psi\longrightarrow
     P: \eta^*\bar\psi\G0\quad
     T: -\bar\psi\G1\G3\quad
     C: \ii\bar\psi^*\G2=-\ii\trans{(\G0\G2\psi)}$\\
\end{tabular}
\end{rightnote}

\begin{tabular}{l@{ :\ \ \ }l}
Electromagnetic Fields & $A^\mu=(\phi,\vc A)$
 \note{We can invert the signs, but cannot lower the index.}\\
& $F_{\mu\nu} =\pmat{0 & & \vc E & \\ & 0 & -B_3 & B_2 \\ -\vc E&B_3&0&-B_1\\&-B_2&B_1&0}$\\
& $F_{\mu\nu}F^{\mu\nu} = -2\left(\vnorm E^2-\vnorm B^2\right)$
\end{tabular}

\subsubsection{Dirac Field Techniques}
\begin{tabular}{l@{ :\ \ \ }l}
Dirac Equations & $(\slashed p-m)u^s(p)=0;\quad(\slashed p+m)v^s(p)=0$\\
&$\bar u^s(p)(\slashed p-m)=0;\quad \bar v^s(p)(\slashed p+m)=0$\\
Dirac Components &
   $\bar u^r(p)u^s(p)=2m\delta^{rs};\quad
    u^{r\dagger}(p) u^s(p)=2E_\vc p\delta^{rs}$\\
 &  $\bar v^r(p)v^s(p)=-2m\delta^{rs};\quad
    v^{r\dagger}(p) v^s(p)=2E_\vc p\delta^{rs};\qquad
    \bar u^r(p)v^s(p)=\bar v^r(p)u^s(p)=0$\\
Spin Sums & $\displaystyle
             \sum\s{spin}u^s(p)\bar u^s(p)=\slashed p+m;\quad
             \sum\s{spin}v^s(p)\bar v^s(p)=\slashed p-m$\\
\end{tabular}

\subsubsection{CPT Table}
\begin{tabular}[t]{c|c|c|cccccc}
 & $\phi$ & $A^\mu$
 & $\bar\psi\psi$ & $\bar\psi\Gm\psi$ & $\bar\psi\Smn\psi$
 & $\bar\psi\Gm\G5\psi$ & $\ii\bar\psi\G5\psi$ & $\Pm$\\\hline
$P$
  & $\eta\phi$ & $\eta$$-$$+$$+$$+$$A^\mu$
  &$+$&$+$$-$$-$$-$&($+$$-$$-$$-$)($+$$-$$-$$-$)&$-$$+$$+$$+$&$-$&$+$$-$$-$$-$\\
$T$
  & $\zeta\phi$ & $\zeta$$+$$-$$-$$-$$A^\mu$
  &$+$&$+$$-$$-$$-$&$-$($+$$-$$-$$-$)($+$$-$$-$$-$)&$+$$-$$-$$-$&$-$&$-$$+$$+$$+$\\
$C$
  & $\xi\phi^*$ & $\xi$$+$$A^{\mu*}$
  &$+$&$-$&$-$&$+$&$+$&$+$\\
\end{tabular}\vspace{.5zw}

($\eta\zeta\xi=1$;
 especially, photon $A^\mu$ is $(\eta,\zeta,\xi)=(-,+,-)$. )

\subsubsection{Polarization Sum}

\subparagraph{Single photon case}$M=\epsilon_\mu^*(k)M^{\mu}$\par
When Ward identity $k_\mu M^\mu=0$ is valid,
\begin{equation}
   \sum\s{pol.}\left|M\right|^2
= \sum\s{pol.}\epsilon_\mu^*(k)\epsilon_\nu(k)M^{\mu}M^{\nu*}
=             \Hmnd M^{\mu}M^{\nu*}
\end{equation}

\subparagraph{Double photons case}$M=\epsilon_\mu^*(k)\epsilon_\nu'^*(k')M^{\mu\nu}$\par
When $k_\mu M^{\mu\nu}=k'_\nu M^{\mu\nu}=0$ is valid,
\begin{equation}
  \sum\s{pol.}\left|M\right|^2
= \sum\s{pol.}
\epsilon_\mu^*(k)\epsilon_\rho(k)\epsilon_\nu'^*(k')\epsilon_\sigma'(k')
[M^{\mu\nu}M^{\rho\sigma*}
= \Hmrd\Hnsd M^{\mu\nu}M^{\rho\sigma*}
\end{equation}
\note{See Sec.~\ref{Sec:Verbose:PolarizationSum} for verbose information.}

\subsection{Dirac's Gamma Algebras}
\subparagraph{Traces}
\begin{align}
 \Tr(\text{any odd \# of $\gamma$'s})&=0\\
 \Tr(\Gm\Gn)&= 4\Hmn\\
 \Tr(\Gm\Gn\Gr\Gs) &= 4(\Hmn\Hrs-\Hmr\Hns+\Hms\Hnr)\\
 \Tr(\text{$\G5$ and any odd \# of $\gamma$'s})&=0\\
 \Tr(\Gm\Gn\G5)&= 0\\
 \Tr(\Gm\Gn\Gr\Gs\G5) &= -4\ii\epsilon^{\mu\nu\rho\sigma}\\
\intertext{Generally, for some $\gamma$-matrices $A,B,C,\dots$,}\quad
\Tr(ABCDEF\cdots) &=
\Minkow{AB}\Tr(CDEF\cdots) - \Minkow{AC}\Tr(BDEF\cdots)\notag\\
& + \Minkow{AD}\Tr(BCEF\cdots) - \Minkow{AE}\Tr(BCDF\cdots) + \cdots\\[1.5zw]
\Tr(ABCDEF\cdots\G5) &=
  \Minkow{AB}\Tr(CDEF\cdots\G5) - \Minkow{AC}\Tr(BDEF\cdots\G5)\notag+\cdots\\
&+ \Minkow{BC}\Tr(ADEF\cdots\G5) - \Minkow{BD}\Tr(ACEF\cdots\G5)\notag+\cdots\\
&+ \Minkow{CD}\Tr(ABEF\cdots\G5) - \Minkow{CE}\Tr(ABDF\cdots\G5)\notag+\cdots\\
&+ \cdots
\end{align}
To prove the second equation, we use following technique:
\begin{equation}
 \Tr(\Gm\Gn\Gr\Gs\cdots)=\Tr(\cdots\Gs\Gr\Gn\Gm);\qquad
 \Tr(\Gm\Gn\Gr\Gs\cdots\G5)=\Tr(\G5\cdots\Gs\Gr\Gn\Gm)
\end{equation}

\subparagraph{Contractions}
\begin{align}
 \Gm\Gmd&=4\\
 \Gm\Gn\Gmd&=-2\Gn\\
 \Gm\Gn\Gr\Gmd&=4\Hnr\\
 \Gm\Gn\Gr\Gs\Gmd&=-2\Gs\Gr\Gn
\end{align}
Generally, for some $\gamma$-matrices $A,B,C,\dots$,
\begin{align}
\text{ODD \# :\quad}&\Gm ABC\cdots \Gmd = -2(\cdots CBA)\\
\text{EVEN \# :\quad}&\Gm ABC\cdots \Gmd = \Tr(ABC\cdots)-\Tr(ABC\cdots\G5)\cdot\G5
\end{align}

\subparagraph{Contractions of $\epsilon$'s}
\begin{align}
& \epsilon^{\alpha\beta\gamma\delta}\epsilon_{\alpha\beta\gamma\delta}=-24;\quad
 \epsilon^{\alpha\beta\gamma\mu}\epsilon_{\alpha\beta\gamma\nu}=-6\delta^\mu_\nu;\quad
 \epsilon^{\alpha\beta\mu\nu}\epsilon_{\alpha\beta\rho\sigma}=-2(
\delta^\mu_\rho\delta^\nu_\sigma-\delta^\mu_\sigma\delta^\nu_\rho
)\\
&\epsilon^{\mu\alpha\beta\gamma}\epsilon_{\mu\alpha'\beta'\gamma'}=-
\left
(\delta^\alpha_{\alpha'}\delta^\beta_{\beta'}\delta^\gamma_{\gamma'}
+\delta^\alpha_{\beta'}\delta^\beta_{\gamma'}\delta^\gamma_{\alpha'}
+\delta^\alpha_{\gamma'}\delta^\beta_{\alpha'}\delta^\gamma_{\beta'}
-\delta^\alpha_{\alpha'}\delta^\beta_{\gamma'}\delta^\gamma_{\beta'}
-\delta^\alpha_{\beta'}\delta^\beta_{\alpha'}\delta^\gamma_{\gamma'}
-\delta^\alpha_{\gamma'}\delta^\beta_{\beta'}\delta^\gamma_{\alpha'}
\right)
\end{align}

$(p\cdot\sigma)(p\cdot\bar\sigma)=p^2$
\begin{itemize}
 \item Fierz Transf.
 \item Noether current
 \item Gordon Id.
 \item Majorana Ferminos
 \item 
 \item Feynman Rules(A.1)
 \item Gamma Algebras(A.3)
 \item A.4, A.5
\end{itemize}

%%% Local Variables:
%%% TeX-master: CheatSheet.tex
%%% End:
