%#!latexmk CheatSheet.tex
%%% Time-Stamp: <2010-11-05 01:58:21 misho>
%%% ï∂éöÉRÅ[ÉhÇÕShift-JISÇ≈Ç∑ÇÊÇÀ

\section{Supersymmetry for $\eta=\diag(+,-,-,-)$}
\subsection{Spinor Convention}
\begin{tabular}{l@{ :\ \ \ }l}
$\epsilon$ tensor
  &$\epsilon^{12}=\epsilon^{\dot1\dot2}=\epsilon_{21}=\epsilon_{\dot2\dot1}=1$
   \qquad{\footnotesize (definition)}\\
Sum Rule & ${}^\alpha{}_{\alpha}$ and ${}_\dalpha{}^{\dalpha}$, except for
  \quad
  $\xi_\alpha=\epsilon_{\alpha\beta}\xi^\beta,\quad
   \xi^\alpha=\epsilon^{\alpha\beta}\xi_\beta,\quad
   \xi_\dalpha=\epsilon_{\dalpha\dbeta}\xi^\dbeta,\quad
   \xi^\dalpha=\epsilon^{\dalpha\dbeta}\xi_\dbeta$.\\[.5zw]
Lorentzïœä∑&
  $\psi'_\alpha = \Lambda\T_\alpha^\beta\psi_\beta,\quad
   \bar\psi'_\dalpha = \bar\psi_\dbeta\Lambda^\dagger\T^\dbeta_\dalpha,\quad
   \psi'^\alpha = \psi^\beta\Lambda^{-1}\T_\beta^\alpha,\quad
   \bar\psi'^\dalpha = (\Lambda^{-1})^\dagger\T^\dalpha_\dbeta\bar\psi'^\dbeta.
  $\\[.5zw]
$\sigma$ matrices& $
 (\Sm)_{\alpha\dbeta} := (1,\vc\sigma)_{\alpha\dbeta},\quad
 (\bSm)^{\dalpha\alpha} :=\epsilon^{\dalpha\dbeta}\epsilon^{\alpha\beta}(\Sm)_{\beta\dbeta}
 =(1,-\vc\sigma)^{\dalpha\beta}$.
\end{tabular}
\begin{flushright}
{\footnotesize (See App.~\ref{sec:verbose-lorentz-group} for a verbose explanation.)}
\end{flushright}
\vspace{-3zw}

\subsection{Spinor Calculation Cheatsheet}
\begin{preposition}{}\vspace{-.5zw}
\begin{align*}
 \eta = (+,-,-,-),\qquad\epsilon^{0123}=-\epsilon_{0123} = 1
\end{align*}\vspace{-3zw}
\begin{align*}
  \epsilon^{12}=\epsilon_{21}=\epsilon^{\dot1\dot2}=\epsilon_{\dot2\dot1}&=1,&
\xi^\alpha&:=\epsilon^{\alpha\beta}\xi_\beta,& \xi_\alpha&=\epsilon_{\alpha\beta}\xi^\beta,&
\bar\xi^\dalpha&:=\epsilon^{\dalpha\dbeta}\bar\xi_\dbeta,& \bar\xi_\dalpha&=\epsilon_{\dalpha\dbeta}\bar\xi^\dbeta
\end{align*}\vspace{-3zw}
\begin{align*}
  \bSm{}^{\dalpha\alpha} &:= \epsilon^{\alpha\beta}\epsilon^{\dalpha\dbeta}\Sm_{\beta\dbeta}&
 \Sm_{\alpha\dalpha}&= \epsilon_{\alpha\beta}\epsilon_{\dalpha\dbeta}\bSm{}^{\dbeta\beta},&
 \Sm:=(1,\vc\sigma),\quad\bSm:=(1,-\vc\sigma)
\end{align*}\vspace{-3zw}
\begin{align*}
  (\Smn)\T_\alpha^\beta:=\tfrac14\left(\Sm\bSn-\Sn\bSm\right)\T_{\alpha}^\beta,\quad
 (\bSmn)\T^\dalpha_\dbeta:=\tfrac14\left(\bSm\Sn-\bSn\Sm\right)\T^{\dalpha}_\dbeta =
(\Snm)^\dagger{}\T^\dalpha_\dbeta.
\end{align*}\vspace{-3zw}
\end{preposition}\vspace{-1.2zw}

\begin{align*}
&\theta^\alpha\theta^\beta=-\tfrac12\epsilon^{\alpha\beta}\thth&
&\theta_\alpha\theta_\beta=\tfrac12\epsilon_{\alpha\beta}\thth&
&(\theta\phi)(\theta\psi)=-\tfrac12(\psi\phi)(\thth)&
(\theta\Sn\btheta)\theta^\alpha &= \tfrac12\thth(\btheta\bSn)^\alpha
\\
&\btheta^\dalpha\btheta^\dbeta=\tfrac12\epsilon^{\dalpha\dbeta}\bthth&
&\btheta_\dalpha\btheta_\dbeta=-\tfrac12\epsilon_{\dalpha\dbeta}\bthth&
&(\btheta\bar\phi)(\btheta\bar\psi)=-\tfrac12(\bar\psi\bar\phi)(\bthth)&
 (\theta\Sn\btheta)\btheta_\dalpha&= -\tfrac12\bthth(\theta\Sm)_\dalpha
\\
&\theta\Sm\bSn\theta=\Hmn\thth&
&\btheta\bSm\Sn\btheta=\Hmn\bthth&
&(\theta\Sm\btheta)(\theta\Sn\btheta)=\tfrac12\thth\bthth\eta^{\mu\nu}&
 (\Sm\btheta)_\alpha(\theta\Sn\btheta) &= \tfrac12(\Sm\bSn\theta)_\alpha\bthth
\end{align*}
\vspace{-2zw}
\begin{align*}
 &\Sm\bSn=\Hmn+2\Smn&
 &\Sm\bSr\Sn+\Sn\bSr\Sm=2\left(\Hmr\Sn+\Hnr\Sm-\Hmn\Sr\right)\\
 &\bSm\Sn=\Hmn+2\bSmn&
 &\bSm\Sr\bSn+\bSn\Sr\bSm=2\left(\Hmr\bSn+\Hnr\bSm-\Hmn\bSr\right)\\
 &\Smn=-\Snm&
 &\Sm\bSn\Sr-\Sr\bSn\Sm=2\ii\epsilon^{\mu\nu\rho\sigma}\Ssd\\
 &\bSmn=-\bSnm&
 &\bSm\Sn\bSr-\bSr\Sn\bSm=-2\ii\epsilon^{\mu\nu\rho\sigma}\bSsd\\
 &\Tr\bSm\Sn=\Tr\Sm\bSn=2\Hmn&
 &\Tr\Smn\Srs=-\tfrac12\left(\Hmr\Hns-\Hms\Hnr\right)+\tfrac\ii2\epsilon^{\mu\nu\rho\sigma}\\
 &\Tr\Smn=\Tr\bSmn=0&
&\Tr\bSmn\bSrs=-\tfrac12\left(\Hmr\Hns-\Hms\Hnr\right)-\tfrac\ii2\epsilon^{\mu\nu\rho\sigma}&
\\
&\Sm_{\alpha\dalpha}\bSmd^{\dbeta\beta}=2\delta^\beta_\alpha\delta^\dbeta_\dalpha&
&\Sm_{\alpha\dalpha}\Sn_{\beta\dbeta}-\Sn_{\alpha\dalpha}\Sm_{\beta\dbeta}
   = 2\left[(\Smn\epsilon)_{\alpha\beta}\epsilon_{\dalpha\dbeta}
           +(\epsilon\bSmn)_{\dalpha\dbeta}\epsilon_{\alpha\beta}\right]&
\\
&\Sm_{\alpha\dalpha}\Smd{}_{\beta\dbeta}=2\epsilon_{\alpha\beta}\epsilon_{\dalpha\dbeta}&
&\Sm_{\alpha\dalpha}\Sn_{\beta\dbeta}+\Sn_{\alpha\dalpha}\Sm_{\beta\dbeta}
   = \Hmn\epsilon_{\alpha\beta}\epsilon_{\dalpha\dbeta}
      - 4\Hrsd(\Srm\epsilon)_{\alpha\beta}(\epsilon\bSsn)_{\dalpha\dbeta}&
\\
&\bSm{}^{\dalpha\alpha}\bSmd^{\dbeta\beta}=2\epsilon^{\alpha\beta}\epsilon^{\dalpha\dbeta}&
&\epsilon_{\dbeta\dalpha}\bSm{}^{\dalpha\alpha}=\epsilon^{\alpha\beta}\Sm_{\beta\dbeta}
\qquad\qquad
\epsilon^{\mu\nu\rho\sigma}\sigma_{\rho\sigma}=2\ii\Smn&
\\
&\sigma\T^\mu^\nu_\alpha^\beta\epsilon_{\beta\gamma} =
 \sigma\T^\mu^\nu_\gamma^\beta\epsilon_{\beta\alpha}&
&\epsilon_{\beta\alpha}\bSm{}^{\dalpha\alpha}=\epsilon^{\dalpha\dbeta}\Sm_{\beta\dbeta}
\qquad\qquad
\epsilon^{\mu\nu\rho\sigma}\bar\sigma_{\rho\sigma}=-2\ii\bSmn
\end{align*}
\vspace{-2.5zw}
\begin{align*}
 \bar\xi\bSm\chi&=-\chi\Sm\bar\xi=(\bar\chi\bSm\xi)^*=-(\xi\Sm\bar\chi)^*&
 (\psi\phi)\chi_\alpha&=-(\phi\chi)\psi_\alpha-(\chi\psi)\phi_\alpha
\\
 \xi\Sm\bSn\chi&=\chi\Sn\bSm\xi=(\bar\chi\bSn\Sm\bar\xi)^*=(\bar\xi\bSm\Sn\bar\chi)^*&
 (\psi\phi)\bar\chi_\dalpha&=\tfrac12(\phi\Sm\bar\chi)(\psi\Smd)_\dalpha
\end{align*}
In the following equations, we chose left-differential notation.
\begin{align*}
 \epsilon^{\alpha\beta}\pbib{}{\theta^\beta}&=-\pbib{}{\theta_\alpha}&
 \pbib{}{\theta^\alpha}\thth&=2\theta_\alpha&
 \epsilon^{\alpha\beta}\pbib{}{\theta^\alpha}\pbib{}{\theta^\beta}\thth &= 4\\
 \epsilon_{\alpha\beta}\pbib{}{\theta_\beta}&=-\pbib{}{\theta^\alpha}&
 \pbib{}{\theta_\alpha}\thth&=-2\theta^\alpha&
 \epsilon_{\alpha\beta}\pbib{}{\theta_\alpha}\pbib{}{\theta_\beta}\thth &= -4\\
 \epsilon^{\dalpha\dbeta}\pbib{}{\btheta^\dbeta}&=-\pbib{}{\btheta_\dalpha}&
 \pbib{}{\btheta^\dalpha}\bthth&=-2\btheta_\dalpha&
 \epsilon_{\dalpha\dbeta}\pbib{}{\btheta_\dalpha}\pbib{}{\btheta_\dbeta}\bthth &= 4\\
 \epsilon_{\dalpha\dbeta}\pbib{}{\btheta_\dbeta}&=-\pbib{}{\btheta^\dalpha}&
 \pbib{}{\btheta_\dalpha}\bthth&=2\btheta^\dalpha&
 \epsilon^{\dalpha\dbeta}\pbib{}{\btheta^\dalpha}\pbib{}{\btheta^\dbeta}\bthth &= -4
\end{align*}

\subsection{General Relations}
\vspace{-2.6zw}
\begin{center}
\hskip3zw (Note: $P_\mu = \ii\Pm$ in our convention.)
\end{center}
\vspace{-1zw}
\begin{align*}
 Q_\alpha       &:=\pbib{}{\theta^\alpha}+\ii(\Sm\btheta)_\alpha\Pm,&
 D_\alpha       &:=\pbib{}{\theta^\alpha}-\ii(\Sm\btheta)_\alpha\Pm,&
 y   &:= x - \ii\theta\sigma\btheta,\\
 \bar Q_\dalpha &=-\pbib{}{\btheta^\dalpha}-\ii(\theta\Sm)_\dalpha\Pm,&
 \bar D_\dalpha &=-\pbib{}{\btheta^\dalpha}+\ii(\theta\Sm)_\dalpha\Pm,&
 y^\dagger      &= x + \ii\theta\sigma\btheta
\end{align*}\vspace{-2zw}
\begin{align*}
 \{Q_\alpha,\bar Q_\dalpha\}&= -2\ii\Sm_{\alpha\dalpha}\Pm,&
 \{D_\alpha,\bar D_\dalpha\}&= 2\ii\Sm_{\alpha\dalpha}\Pm,&
 \text{(others)} &=0.
\end{align*}\vspace{-2zw}
\begin{align*}
&\bar D_\dalpha(y,\theta,\btheta)        = -\pbib{}{\btheta^\dalpha}&
&     D_\alpha (y,\theta,\btheta)        = \pbib{}{\theta^\alpha} - 2\ii(\Sm\btheta)_\alpha\pbib{}{y^\mu}
\\
&     D_\alpha(y^\dagger,\theta,\btheta) = \pbib{}{\theta^\alpha}&
&\bar D_\dalpha(y^\dagger,\theta,\btheta)= -\pbib{}{\btheta^\dalpha}+2\ii(\theta\Sm)_\dalpha\pbib{}{(y^\dagger)^\mu}
\\
&\bar D^\dalpha(y,\theta,\btheta) = \pbib{}{\btheta_\dalpha}&
\\
&     D^\alpha(y^\dagger,\theta,\btheta) = -\pbib{}{\theta_\alpha}&
&     D^\alpha(y,\theta,\btheta)         = -\pbib{}{\theta_\alpha}+2\ii(\btheta\bSm)^\alpha\pbib{}{y^\mu}
\end{align*}

\begin{align}
 \phi(y)
&&=&&&{} \phi(x) - \ii\theta\Sm\btheta\Pm\phi(x)-\frac14\thth\bthth\Psq\phi(x)&&
 ={}&& \phi(y^\dagger)  -2\ii\theta\Sm\btheta\Pm\phi(y^\dagger)-\thth\bthth\Psq\phi(y^\dagger)\\
 \phi(y^\dagger)
&&=&&&{} \phi(x) + \ii\theta\Sm\btheta\Pm\phi(x)-\frac14\thth\bthth\Psq\phi(x)&&
={}&& \phi(y) + 2\ii\theta\Sm\btheta\Pm\phi(y)-\thth\bthth\Psq\phi(y)\\
 \phi(x)
&&=&&&{} \phi(y) + \ii\theta\Sm\btheta\Pm\phi(y)-\frac14\thth\bthth\Psq\phi(y)&&
={}&& \phi(y^\dagger) - \ii\theta\Sm\btheta\Pm\phi(y^\dagger)-\frac14\thth\bthth\Psq\phi(y^\dagger)
\end{align}

\subsection{Conventions}
\begin{center}
 \begin{tabular}[t]{l|c|l}
 Martin (SUSY Primer) &  $\epsilon_\alpha = \sqrt2\xi_\alpha$ & Wess\&Bagger (SUSY and SUGRA)\\\hline
 $\delta \phi = \epsilon \psi$ & same & $\delta A=\sqrt2\xi \psi$\\
 $\delta \psi_\alpha = \ii(\Sm\epsilon^\dagger)_\alpha\Dm\phi + \epsilon_\alpha F$ & same &
 $\delta \psi        = \ii\sqrt2\Sm\ol\xi\Dm A + \sqrt2\xi F$\\
 $\delta F = \ii\epsilon^\dagger\bSm\Dm\psi+\sqrt2g(T^a\phi)\epsilon^\dagger\lambda^{\dagger a}$
&&\\\hline
 $\delta A_\mu = \frac1{\sqrt2}\left(\epsilon^\dagger\bSm\lambda^a+\lambda^{\dagger a}\bSm\epsilon\right)$
 &$\lambda\s{M}=\ii\lambda\s{WB}$&
 $\delta v_\mu = \ii\left(\xi^\dagger \bSm\lambda^a-\lambda^\dagger\bSm\xi\right)$\\
 $\delta\lambda=\frac{\ii}{2\sqrt2}(\Sm\Sn\epsilon)F_{\mu\nu}+\frac1{\sqrt2}\epsilon D$
 &&\\
 $\delta D = \frac{\ii}{\sqrt2}\left(\epsilon^\dagger\bSm\Dm\lambda-\Dm\lambda^\dagger\bSm\epsilon\right)$
 \end{tabular}
\end{center}

\newpage
\subsection{Chiral Superfields : $\bar D_\dalpha \Phi = 0$}
\subparagraph{Explicit Expression}
\begin{align}
\Phi
={}& \phi(y) + \sqrt2\theta\psi(y)+\thth F(y)\\
={}& \phi(x) - \ii\theta\Sm\btheta\Pm\phi(x)
               - \frac14\thth\bthth\Psq\phi(x)
     + \sqrt2\theta\psi(x) - \frac\ii{\sqrt2}\thth\btheta\bSm\Pm\psi(x)
     + \thth F(x)\\
={}& \phi(y^\dagger) - 2\ii\theta\Sm\btheta\Pm\phi(y^\dagger)
               - \thth\bthth\Psq\phi(y^\dagger)
     + \sqrt2\theta\psi(y^\dagger) - \sqrt2\ii\thth\btheta\bSm\Pm\psi(y^\dagger)
     + \thth F(y^\dagger)\\
\Phi^\dagger
={}& \phi^*(y^\dagger) + \sqrt2\btheta\bar\psi(y^\dagger)+\bthth F^*(y^\dagger)\\
={}& \phi^*(x) + \ii\theta\Sm\btheta\Pm\phi^*(x)
               - \frac14\thth\bthth\Psq\phi^*(x)
   + \sqrt2\btheta\bar\psi(x) - \frac\ii{\sqrt2}\bthth\theta\Sm\Pm\bar\psi(x)
   + \bthth F^*(x)\\
={}& \phi^*(y) + 2\ii\theta\Sm\btheta\Pm\phi^*(y)
               - \thth\bthth\Psq\phi^*(y)
   + \sqrt2\btheta\bar\psi(y) - \sqrt2\ii\bthth\theta\Sm\Pm\bar\psi(y)
   + \bthth F^*(y)
\end{align}

\subparagraph{Product of Chiral Superfields}
\begin{align}
\Phi^\dagger_i\Phi_j(x,\theta,\btheta)
={}& \phi^*_i\phi_j
       + \sqrt2\phi^*_i\theta\psi_j + \sqrt2\btheta\bar\psi_i\phi_j
       + \thth \phi^*_iF_j + \bthth F^*_i\phi_j\notag\\
   & - \ii\theta\Sm\btheta\left(\phi^*_i\Pm\phi_j-\Pm\phi^*_i\phi_j\right)
       + 2\btheta\bar\psi_i\theta\psi_j\notag\\
   & + \frac\ii{\sqrt2}\thth
         \left(\phi^*_i\Pm\psi_j-\Pm\phi^*_i\psi_j\right)\Sm\btheta
       + \sqrt2\thth \btheta\bar\psi_i F_j\notag\\
   & - \frac\ii{\sqrt2}\bthth\theta\Sm
         \left(\Pm\bar\psi_i\phi_j-\bar\psi_i\Pm\phi_j\right)
       + \sqrt2\bthth F^*_i\theta\psi_j\\
   & + \thth\bthth\left[
        F^*_iF_j-\frac14\phi^*_i\Psq\phi_j-\frac14\Psq\phi^*_i\phi_j
        +\frac12\Pm\phi^*_i\Pm\phi_j
        - \frac\ii2\Pm\bar\psi_i\bSm\psi_j
        + \frac\ii2\bar\psi_i\bSm\Pm\psi_j\right]\notag\\
\leadsto{}
   & \phi^*_i\phi_j
       + \sqrt2\phi^*_i\theta\psi_j + \sqrt2\btheta\bar\psi_i\phi_j
       + \thth \phi^*_iF_j + \bthth F^*_i\phi_j\notag\\
   & - 2\ii(\theta\Sm\btheta)(\phi^*_i\Pm\phi_j)
       + \sqrt2\ii\thth(\Pm\phi^*_i)\btheta\bSm\psi_j
       + \sqrt2\ii\bthth\theta\Sm\bar\psi_i\Pm\phi_j\\
   & + 2\btheta\bar\psi_i\theta\psi_j
       + \sqrt2\thth \btheta\bar\psi_i F_j
       + \sqrt2\bthth F^*_i\theta\psi_j\notag\\
   & + \thth\bthth\left[
        F^*_iF_j + \Pmu\phi^*_i\Pm\phi_j + \ii\bar\psi_i\bSm\Pm\psi_j\right]\notag
\end{align}\vspace{-2zw}
\begin{align}
\Phi_i\Phi_j\text{(in $y$-basis)}
={}& \phi_i\phi_j+\sqrt2\theta\left[\psi_i\phi_j+\phi_i\psi_j\right]
     +\thth\left[\phi_iF_j+F_i\phi_j-\psi_i\psi_j\right]\\
\Phi_i\Phi_j\Phi_k\text{(in $y$-basis)}
={}& \phi_i\phi_j\phi_k
     + \sqrt2\theta\left[\psi_i\phi_j\phi_k
                        +\phi_i\psi_j\phi_k
                        +\phi_i\phi_j\psi_k\right]\notag\\
   & +\thth\left[
      F_i\phi_j\phi_k+\phi_iF_j\phi_k+\phi_i\phi_jF_k
      -\psi_i\psi_j\phi_k-\psi_i\phi_j\psi_k
      -\phi_i\psi_j\psi_k
      \right]
\end{align}\vspace{-3zw}\par
\begin{flushright}\footnotesize
(Products of chiral superfields are still chiral superfields.)
\end{flushright}
\begin{equation}
 \ee^{\ii k \Phi}=\ee^{\ii k \phi(y)}\left[1+\ii k\left(\sqrt2\theta\phi(y)+\thth F(y)\right)+\frac{k^2}2\thth\psi(y)\psi(y)\right]
\end{equation}
\subparagraph{Lagrangian Blocks}
\begin{align}
 \mathcal L\s{kin.}
={}& \Phi^\dagger_i\Phi_j\Big|_{\thth\bthth}
=  F^*_iF_j + \Pmu\phi^*_i\Pm\phi_j + \ii\bar\psi_i\bSm\Pm\psi_j\\
 \mathcal L\s{super}
={}& W\Big|_{\thth} + W^*\Big|_{\bthth}
= \int\dd^2\theta
     \left[\lambda_i\Phi_i + m_{ij} \Phi_i\Phi_j
                           + y_{ijk}\Phi_i\Phi_j\Phi_k\right]+\Hc\notag\\
={}& \lambda_iF_i + m_{ij}\left(\phi_iF_j+F_i\phi_j-\psi_i\psi_j\right)
    +y_{ijk}\Bigl[\left(F_i\phi_j\phi_k-\psi_i\psi_j\phi_k\right)+\text{($jki$ and $kij$ terms)}\Bigr]
\end{align}




\subsection{Vector Superfields and Gauge Theory : $V=V^\dagger$}
\subsubsection{Abelian Case --- Field Construction}
\subparagraph{Explicit Expression}
\begin{align}
 V
={}& C(x) + \ii\theta\chi(x) - \ii\btheta\bar\chi(x)\notag
 \\& + \frac\ii2\thth\left[M(x)+\ii N(x)\right]
     - \frac\ii2\bthth\left[M(x)-\ii N(x)\right]
     - \theta\Sm\btheta A_\mu(x)\notag
 \\& + \ii\thth\btheta\left[\bar\lambda(x)-\frac\ii2\bSm\Pm\chi(x)\right]
     - \ii\bthth\theta\left[\lambda(x)-\frac\ii2\Sm\Pm\bar\chi(x)\right]
     + \frac12\thth\bthth\left[D(x)-\frac12\Psq C(x)\right] \\
={}& C(y) + \ii\theta\chi(y) - \ii\btheta\bar\chi(y)\notag
 \\& + \frac\ii2\thth\left[M(y)+\ii N(y)\right]
     - \frac\ii2\bthth\left[M(y)-\ii N(y)\right]
     - \theta\Sm\btheta \left[A_\mu(y)-\ii\Pm C(y)\right]\notag
 \\& + \ii\thth\btheta\bar\lambda(y)
     - \ii\bthth\theta\left[\lambda(y)-\ii\Sm\Pm\bar\chi(y)\right]
     + \frac12\thth\bthth\left[D(y)-\Psq C(y)-\ii\Pm A^\mu(y)\right] \\
={}& C(y^\dagger) + \ii\theta\chi(y^\dagger) - \ii\btheta\bar\chi(y^\dagger)\notag
 \\& + \frac\ii2\thth\left[M(y^\dagger)+\ii N(y^\dagger)\right]
     - \frac\ii2\bthth\left[M(y^\dagger)-\ii N(y^\dagger)\right]
     - \theta\Sm\btheta \left[A_\mu(y^\dagger)+\ii\Pm C(y^\dagger)\right]\notag
 \\& + \ii\thth\btheta\left[\bar\lambda(y^\dagger)-\ii\bSm\Pm\chi(y^\dagger)\right]
     - \ii\bthth\theta\lambda(y^\dagger)
     + \frac12\thth\bthth\left[D(y^\dagger)-\Psq C(y^\dagger)+\ii\Pm A^\mu(y^\dagger)\right]
\end{align}
\subparagraph{Supersymmetric Gauge Transformation :  $V \rightarrow V+\Phi + \Phi^\dagger$}
\begin{align}
C       &\to C+(\phi+\phi^*)      & A_\mu  &\to A_\mu + \ii\Pm(\phi-\phi^*)\notag\\
\chi    &\to \chi - \ii\sqrt2\psi & \lambda&\to \lambda\\
M+\ii N &\to M + \ii N - 2\ii F   & D      &\to D\notag
\end{align}

\subparagraph{Wess-Zumino Gauge} $C=\chi=M=N=0$\par
Fixing this gauge breaks SUSY, but still allows the usual gauge transformation
\begin{equation}
 A_\mu \to A_\mu + \Pm \alpha,\ \ \lambda\to\lambda,\ \ D\to D.
\end{equation}
\begin{align*}
 V  &= - \theta\Sm\btheta A_\mu(x) + \ii\thth\btheta\bar\lambda(x)
       - \ii\bthth\theta\lambda(x) + \dfrac12\thth\bthth D(x) &
V^2 &=\dfrac12\thth\bthth A_\mu A^\mu
\\
    &= - \theta\Sm\btheta A_\mu(y) + \ii\thth\btheta\bar\lambda(y) - \ii\bthth\theta\lambda(y) + \dfrac12\thth\bthth \left[D(y)-\ii\Pm A^\mu(y)\right]&
V^3 &= 0
\\
    &= - \theta\Sm\btheta A_\mu(y^\dagger) + \ii\thth\btheta\bar\lambda(y^\dagger) - \ii\bthth\theta\lambda(y^\dagger) + \dfrac12\thth\bthth \left[D(y^\dagger)+\ii\Pm A^\mu(y^\dagger)\right]
\\
 \ee^{kV}&=1- k\theta\Sm\btheta A_\mu(x) + k\ii\thth\btheta\bar\lambda
       - k\ii\bthth\theta\lambda + \thth\bthth\left[\frac{k}2 D + \frac{k^2}4A_\mu A^\mu\right]
\end{align*}

\subparagraph{Field Strength}
\begin{align}
&W_\alpha       =-\frac14\bar D\bar D D_\alpha V,\quad
\bar W_\dalpha =-\frac14 D D \bar D_\dalpha V;\qquad
 W_\alpha \to W_\alpha \quad\text{\footnotesize(gauge invariant)}\\
& \bar D_\dbeta W_\alpha  = D_\beta \bar W_\dalpha = 0;\qquad
  D^\alpha W_\alpha =  \bar D_\dalpha \bar W^\dalpha
\end{align}
\vspace{-4.5zw}\par
\begin{align}
 W_{\alpha}
&=  -\ii\lambda_\alpha(y) + \theta_\alpha D(y) + \ii(\Smn\theta)_\alpha F_{\mu\nu}(y) - \thth\left[\Sm\Pm\bar\lambda(y)\right]_\alpha\\
 \bar W_{\dalpha}
&=  \ii\bar\lambda_\dalpha(y^\dagger) + \btheta_\dalpha D(y^\dagger) + \ii(\btheta\bSmn)_\dalpha F_{\mu\nu}(y^\dagger) - \bthth\left[\Pm\lambda(y^\dagger)\Sm\right]_\dalpha
\end{align}
\vspace{-4.5zw}\par
\begin{align}
 W^\alpha W_\alpha \big|_{\thth}
=  -\frac14\bar D\bar D W^\alpha D_\alpha V
=  -\frac12F^{\mu\nu}F_{\mu\nu}+\frac\ii4\epsilon^{\mu\nu\rho\sigma}F_{\mu\nu}F_{\rho\sigma}+2\ii\lambda\Sm\Pm\bar\lambda + D^2
\end{align}

\Subparagraph{Lagrangian Blocks}\vspace{-1.1zw}
\begin{flushright}\footnotesize
 ($\Lag\s{inv}$ is SUSY- and gauge-invariant, while $\Lag\s{mass}$ is not gauge-invariant.)
\end{flushright}\vspace{-1.2zw}
\begin{align}
 \mathcal L\s{inv}
&= \frac14\left( W^\alpha W_\alpha\Big|_\thth + \bar W_\dalpha \bar W^\dalpha\Big|_\bthth\right)
 = \frac14\left( W^\alpha D_\alpha V+\bar W_\dalpha \bar D^\dalpha V\right)\Big|_{\thth\bthth}\notag\\
&= -\frac14F^{\mu\nu}F_{\mu\nu}+\ii\lambda\Sm\Pm\bar\lambda + \frac12 D^2\\
 \mathcal L\s{mass}
&= m^2 V^2\Big|_{\thth\bthth}\notag\\
&= m^2\left(\frac12 A^\mu A_\mu + \ii\bar\chi\bSm\Pm\chi - (\lambda\chi+\bar\lambda\bar\chi) + \frac12(M^2+N^2) + CD + \frac12{\Pm C\Pmu C}\right)\notag\\
&= \frac12{\Pm C'\Pmu C'}+ \ii \bar\chi'\bSm\Pm\chi'
   + \frac{m^2}2 A^\mu A_\mu -  m(\lambda\chi'+\bar\lambda\bar\chi') + mC'D + \frac{m^2}{2}(M^2+N^2)
\end{align}

\subsubsection{Abelian Case --- Gauge Theory}\vspace{-2.4zw}
\begin{align}
\Lag&\ni\Phi^\dagger\ee^{2gqV}\Phi;&
 \Phi\to \ee^{\ii q \Lambda}\Phi,\quad& \Phi^\dagger\to \Phi^\dagger\ee^{-\ii q \Lambda^\dagger};& 2gV&\to 2gV-\ii(\Lambda-\Lambda^\dagger)
\end{align}
For gauge transformation $\Lambda=\lambda(y)+\sqrt2\theta\xi(y)+\thth K(y)$,
\begin{align*}
  \phi&\to \ee^{\ii q\lambda}\phi&
  C   &\to C+\tfrac1g\nIm\lambda&
M+\ii N&\to M+\ii N-\tfrac1g K
\\
  \psi&\to \ee^{\ii q\lambda}\left(\psi+\ii q\phi\cdot \xi\right)&
  \chi&\to \chi-\tfrac{1}{\sqrt2g} \xi&
A_\mu &\to A_\mu+\tfrac1g \Pm(\nRe\lambda)
\\
  F   &\to \ee^{\ii q\lambda}\left(F+\ii q\phi K-\ii q \xi\psi +\frac{q^2}{2}\xi\xi\phi\right)&
\lambda&\to\lambda&
D&\to D\\
\end{align*}\vspace{-3.1zw}

Note that $\Dm\phi=(\Pm-\ii g q A_\mu)\phi$ yields from these definitions.\vspace{.8zw}

\Subparagraph{Lagrangian block}\vspace{-2zw}
\begin{align}
 \Lag\s{gauge}&= \frac14 W^\alpha W_\alpha\Big|_\thth + \Hc&&
=-\frac14F^{\mu\nu}F_{\mu\nu}+\ii\lambda\Sm\Pm\bar\lambda + \frac12 D^2\\
 \Lag\s{chiral}&=\Phi^\dagger\ee^{2gqV}\Phi\Big|_{\thth\bthth}&&
=F^*F+\Dm\phi^*\Dmu\phi+\ii\bar\Psi\bSm\Dm\psi + qg D\phi^*\phi+\ii\sqrt2gq\left(\phi^*\lambda\psi-\phi\bar\lambda\bar\psi\right)
\end{align}


\subsubsection{Non-Abelian Case}
\begin{preposition}{}\vspace{-.5zw}
\begin{align*}
 &T^a:\text{generators (Hermitian)};\\
 &\Tr T^aT^b = k\delta^{ab}\ (k>0),&
 &[T^a,T^b]=\ii f^{abc}T^c\ \text{($f$ is anti-symmetric)}
\end{align*}\vspace{-3zw}
\end{preposition}\vspace{.7zw}

Expclicit expression is the same as the Abelian case.

\subparagraph{Supersymmetric Gauge Transformation}
\begin{align}
\Lag\ni\Phi^\dagger\ee^{2g\tilde V}\Phi;
\qquad
 \Phi\to \ee^{\ii\tilde\Lambda}\Phi,\quad
 \Phi^\dagger&\to \Phi^\dagger\ee^{-\ii\tilde\Lambda^\dagger};\qquad
\ee^{2g\tilde V} \to \ee^{-\ii \tilde\Lambda^\dagger}\ee^{2g\tilde V}\ee^{\ii\tilde\Lambda}\\
 &\text{with}\ \tilde V:=V^aT^a,\quad
 \tilde \Lambda := \Lambda^aT^a,\quad
 \tilde \Lambda^\dagger := (\Lambda^a)^\dagger T^a\notag
\end{align}
\begin{align}
 2g\tilde V&\to 2g\tilde V-\ii(\tilde\Lambda-\tilde\Lambda^\dagger)-\frac12\left(
 [\tilde\Lambda,\tilde\Lambda^\dagger]+\ii[2g\tilde V,\tilde\Lambda+\tilde\Lambda^\dagger]\right)+\cdots\\
 &=\left[
 2gV^a-\ii(\Lambda^a-\Lambda^{\dagger a})+\frac12\Bigl(
-\ii\Lambda^b\Lambda^{\dagger c}+2gV^b(\Lambda^c+\Lambda^{\dagger c})\Bigr)f^{abc}+\cdots\right]T^a
\end{align}
We do not present the transformations of the components; note that $\lambda$ and $D$ are transformed in non-Abelian theories.

\Subparagraph{Wess-Zumino Gauge}
 Note that the lowest order term of the gauge transformation is independent of $V$, which guarantees that we can still take the Wess-Zumino gauge.

Here the gauge transformation is restricted as
$\Lambda=\lambda(y) = \lambda(x)-\ii\theta\Sm\btheta\Pm\lambda(x)-\frac14\thth\bthth\Psq\lambda(x)$
: $\lambda\in\Real$.
\begin{align}
 2gV^e&\to
2g\left(
V^e
-f^{eab}\lambda^aV^b
+6f^{abc}f^{ade}V^b\lambda^c\lambda^d
\right)\notag\\
&\qquad\qquad
+\theta\Sm\btheta\left(
-2\Pm\lambda^e
+f^{eab}\lambda^a\Pm\lambda^b
+4f^{acd}f^{abe}\lambda^b\lambda^c\Pm\lambda^d
\right)+\cdots
\\[.5zw]
 A_\mu^e&\to
A_\mu^e
+f^{eab}A_\mu^a\lambda^b
+6f^{abc}f^{ade}A_\mu^b\lambda^c\lambda^d\notag\\
&\qquad\qquad
+\frac1g\left(
\Pm\lambda^e
-\frac12f^{eab}\lambda^a\Pm\lambda^b
-2f^{acd}f^{abe}\lambda^b\lambda^c\Pm\lambda^d
\right)+\cdots
%\\[.5zw]
\end{align}
Note that $C,\chi, M$ and $N$ are kept invariant automatically, for the transformation is held within Wess-Zumino gauge.

\subsection{Gauge Theory}

\newpage


\Paragraph{Field Strength}
Defining all component fields as including generators and coupling
constants,
\begin{align}
 \ee^{\pm2gV^aT^a}
\to{}& \ee^{\pm2V}\notag\\
  ={}& 1 \mp 2\theta\Sm\btheta A_\mu(x)
         \mp 2\ii\left[\bthth\theta\lambda(x)-\thth\btheta\bar\lambda(x)\right]
         + \thth\bthth\left[{\RED -}A^\mu(x) A_\mu(x) - D(x)\right]
\end{align}
Therefore, in $y^+$-basis,
\begin{align}
 D_\alpha\ee^{-2V}
={}&\pbib{}{\theta^\alpha}\Bigl\{
 1 + 2\theta\Sm\btheta A_\mu
   + 2\ii\left[\bthth\theta\lambda-\thth\btheta\bar\lambda\right]
   + \thth\bthth\left[A^\mu A_\mu - D - \ii\Pm
 A^\mu\right]\Bigr\}\notag\\
={}& 2(\Sm\btheta)_\alpha A_\mu
   + 2\ii\bthth\lambda_\alpha - 4\ii\theta_\alpha\btheta\bar\lambda
   + 2\theta_\alpha\bthth\left[A^\mu A_\mu - D - \ii\Pm A^\mu\right]
\end{align}
\begin{align}
 \ee^{2V}D_\alpha\ee^{-2V}
={}&\Bigl\{
 1 - 2\theta\Sm\btheta A_\mu
   - 2\ii\left[\bthth\theta\lambda-\thth\btheta\bar\lambda\right]\Bigr\}D_\alpha\ee^{-2V}\notag\\
={}&
     2(\Sm\btheta)_\alpha A_\mu
   + 2\ii\bthth\lambda_\alpha - 4\ii\theta_\alpha\btheta\bar\lambda
   + 2\theta_\alpha\bthth\left[A^\mu A_\mu - D - \ii\Pm A^\mu\right]\notag\\
   & - 2\theta\Sm\btheta A_\mu\left[
     2(\Sm\btheta)_\alpha A_\mu - 4\ii\theta_\alpha\btheta\bar\lambda
     \right]\notag\\
   & + 2\ii \theta\theta\btheta\bar\lambda\cdot2(\Sm\btheta)_\alpha A_\mu\notag\\
={}& {\RED 2(\Sm\btheta)_\alpha A_\mu - 4\ii\theta_\alpha\btheta\bar\lambda}
     + 2\theta_\alpha\bthth\left[A^\mu A_\mu - D - \ii\Pm A^\mu\right]
     + 2\ii\bthth\lambda_\alpha\notag\\
  &  - 2A_\mu A_\nu\bthth\epsilon_{\alpha\gamma}(\theta\Sm\bSn)^\gamma
     - 4\ii A_\mu\thth\bthth(\Sm\bar\lambda)_\alpha
       \quad\text{\RED (in $y^+$-basis)}\\
={}& {\BLUE 2(\Sm\btheta)_\alpha A_\mu
     - 2\ii\bthth\epsilon_{\alpha\gamma}(\theta\Sn\bSm)^\gamma\Pn A_\mu
     - 4\ii\theta_\alpha\btheta\bar\lambda-2\thth\bthth(\Sm\Pm\bar\lambda)_\alpha}\notag\\
   & + 2\theta_\alpha\bthth\left[A^\mu A_\mu - D - \ii\Pm A^\mu\right]
     + 2\ii\bthth\lambda_\alpha\notag\\
  &  - 2A_\mu A_\nu\bthth\epsilon_{\alpha\gamma}(\theta\Sm\bSn)^\gamma
     - 4\ii A_\mu\thth\bthth(\Sm\bar\lambda)_\alpha\quad\text{\BLUE(in $y$-basis)}
\end{align}
In $y$-basis, $\bar D\bar D = 4\cdot\pbib{}{(\bthth)}$. Therefore,
\begin{align}
 W_\alpha
={}& -\frac14\bar D\bar D\ee^{2V}D_\alpha\ee^{-2V}\\
={}&   2(A_\mu A_\nu+\ii\Pn A_\mu)(\Sn\bSm\theta)_\alpha
     + 2\thth(\Sm\Pm\bar\lambda)_\alpha\notag\\
   & - 2\theta_\alpha\left[A^\mu A_\mu - D - \ii\Pm A^\mu\right]
     - 2\ii\lambda_\alpha + 4\ii A_\mu\thth(\Sm\bar\lambda)_\alpha\quad\text{\BLUE(in $y$-basis)}\\
={}&   2(A_\mu A_\nu+\ii\Pn A_\mu)(\Sn\bSm\theta)_\alpha
     + 2\thth(\Sm\Pm\bar\lambda)_\alpha\notag\\
   & - 2\theta_\alpha\left[A^\mu A_\mu - D - \ii\Pm A^\mu\right]
     - 2\ii\lambda_\alpha + 4\ii A_\mu\thth(\Sm\bar\lambda)_\alpha\notag\\
   & - \ii\thth (\Sn\bSm\Sr\btheta)_\alpha
       (\Pr A_\mu A_\nu + A_\mu\Pr A_\nu + \ii\Pn\Pr A_\mu)\notag\\
   & + \ii\thth (\Sr\btheta)_\alpha
       (\Pr A^\mu A_\mu + A^\mu\Pr A_\mu - \Pr D -\ii\Pm\Pr A^\mu)
       \quad\text{(in $x$-basis)}\\
 W^\alpha
={}&   2(A_\mu A_\nu+\ii\Pn A_\mu)(\theta\Sm\bSn)^\alpha
     - 2\thth(\Pm\bar\lambda\bSm)^\alpha\notag\\
   & - 2\theta^\alpha\left[A^\mu A_\mu - D - \ii\Pm A^\mu\right]
     - 2\ii\lambda^\alpha - 4\ii A_\mu\thth(\bar\lambda\bSm)^\alpha\quad\text{\BLUE(in $y$-basis)}
\end{align}
\newpage
\begin{align}
 W^\alpha W_\alpha\Big|_{\thth}
={}&
4(A_\mu A_\nu+\ii\Pn A_\mu)(A_\rho A_\sigma+\ii\Ps A_\rho)(\theta\Sm\bSn\Ss\bSr\theta)
\notag\\&-4(A_\mu A_\nu+\ii\Pn A_\mu)[A^\mu A_\mu - D - \ii\Pm A^\mu](\theta\Sm\bSn\theta)
\notag\\&+4\ii\thth(\Pm\bar\lambda\bSm\lambda)
\notag\\&-4[A^\mu A_\mu - D - \ii\Pm A^\mu](A_\mu A_\nu+\ii\Pn A_\mu)(\theta\Sn\bSm\theta)
\notag\\&+4\thth[A^\mu A_\mu - D - \ii\Pm A^\mu][A^\mu A_\mu - D - \ii\Pm A^\mu]
\notag\\&+4\ii[A^\mu A_\mu - D - \ii\Pm A^\mu]\theta\lambda
\notag\\&-4\ii(\lambda\Sn\bSm\theta)(A_\mu A_\nu+\ii\Pn A_\mu)
\notag\\&-4\ii\thth(\lambda\Sm\Pm\bar\lambda)
\notag\\&+8\thth\lambda^\alpha A_\mu(\Sm\bar\lambda)_\alpha
\notag\\&-8\thth A_\mu(\bar\lambda\bSm\lambda)\notag\\
={}& 4(\theta\Sm\bSn\Ss\bSr\theta)
     [A_\mu A_\nu+\ii\Pn A_\mu][A_\rho A_\sigma+\ii\Ps A_\rho]
\notag\\&-4(\theta\Sm\bSn\theta)
    \Bigl\{A^\mu A_\mu - D - \ii\Pm A^\mu,A_\mu A_\nu+\ii\Pn A_\mu\Bigr\}
\notag\\&+4\ii\thth(\Pm\bar\lambda\bSm\lambda - \lambda\Sm\Pm\bar\lambda)
\notag\\&+4\thth[A^\mu A_\mu - D - \ii\Pm A^\mu][A^\mu A_\mu - D - \ii\Pm A^\mu]
\notag\\&+8\thth\lambda^\alpha A_\mu(\Sm\bar\lambda)_\alpha
\notag\\&-8\thth A_\mu(\bar\lambda\bSm\lambda)\quad\text{\BLUE(in $y$-basis)}\notag\\
\leadsto{}
  & 4(\Hmn\Hsr-\Hms\Hnr+\Hmr\Hns)
     [A_\mu A_\nu+\ii\Pn A_\mu][A_\rho A_\sigma+\ii\Ps A_\rho]
\notag\\&-4
    \Bigl\{A^\mu A_\mu - D - \ii\Pm A^\mu,A^\nu A_\nu+\ii\Pn A^\nu\Bigr\}
\notag\\&+4[A^\mu A_\mu - D - \ii\Pm A^\mu][A^\mu A_\mu - D - \ii\Pm A^\mu]
\notag\\&+4\ii(\Pm\bar\lambda\bSm\lambda - \lambda\Sm\Pm\bar\lambda)
         + 8\lambda^\alpha A_\mu(\Sm\bar\lambda)_\alpha
         - 8 A_\mu(\bar\lambda\bSm\lambda)\notag\\
={}& -2F^{\mu\nu}F_{\mu\nu} + 4(D+2\ii\Pm A^\mu)(D+2\ii\Pm A^\mu)\notag\\
   & +4\ii(\Pm\bar\lambda\bSm\lambda - \lambda\Sm\Pm\bar\lambda)
     +8\lambda^\alpha A_\mu(\Sm\bar\lambda)_\alpha -8 A_\mu(\bar\lambda\bSm\lambda),\\
\bar W_\dalpha\bar W^\dalpha\Big|_{\bthth}
={}& -2F^{\mu\nu}F_{\mu\nu} + 4(D-2\ii\Pm A^\mu)(D-2\ii\Pm A^\mu)\notag\\
   & +4\ii(\Pm\lambda\Sm\bar\lambda - \bar\lambda\bSm\Pm\lambda)
     +8\bar\lambda^\alpha A_\mu(\bSm\lambda)_\alpha -8 A_\mu(\lambda\Sm\bar\lambda),
\end{align}
where
\begin{equation}
 F_{\mu\nu} = \Pm A_\nu - \Pn A_\mu + \ii[A_\mu,A_\nu]
\end{equation}
Defining the generators as
\footnote{The last one is anomaly-free condition, yielding $\Tr T^aT^bT^c = \ii kgf^{abc}/2$.}
\begin{align}
  {T^a}^\dagger &= T^a,&
  [T^a,T^b] &= \ii f^{abc}T^c,&
  \Tr T^aT^b &= k\delta^{ab}\quad(k>0),&
  \Tr(\{T^a,T^b\}T^c)&=0,
\end{align}
\begin{align}
 \frac{1}{16kg^2}\Tr\left(
 W^\alpha W_\alpha\Big|_{\thth}+\bar W_\dalpha\bar W^\dalpha\Big|_{\bthth}
 \right)
={}& - \frac14 F^{a\mu\nu}F^a_{\mu\nu}
     + \frac12 D^aD^a-2\Pm A^{a\mu}\Pn A^{a\nu}\notag\\
   & - \frac12\ii\left(\lambda\Sm D_\mu\bar\lambda+\bar\lambda\bSm D_\mu\lambda\right)
\end{align}
Here
\begin{align}
  F^a_{\mu\nu} &= \Pm A^a_\nu - \Pn A^a_\mu - f^{abc}A^b_\mu A^c_\nu\\
  D_\mu\lambda^a &= \Pm\lambda^a-gf^{abc}A^b_\mu\lambda^c\\
  D_\mu\bar\lambda^a &= \Pm\bar\lambda^a-gf^{abc}A^b_\mu\bar\lambda^c
\end{align}
\newpage
\paragraph{Interaction Terms}
\begin{equation}
 \ee^{-2gV^aT^a}
  = 1 + 2g\theta\Sm\btheta A^a_\mu T^a
         + 2\ii g\bthth\theta\lambda^aT^a
         - 2\ii g\thth\btheta\bar\lambda^aT^a
         - \thth\bthth\left[g^2A^{a\mu} A^b_\mu T^aT^b + gD^aT^a\right]
\end{equation}
\begin{align}
\Phi^\dagger\ee^{-2gV^aT^a}\Phi\Big|_{\theta^4}
={}& \phi^*\thth\bthth\left[-g^2A^{a\mu} A^b_\mu T^aT^b - gD^aT^a\right]\phi\notag\\
   &   + \sqrt2\phi^*\left[2\ii g\bthth\theta\lambda^aT^a\right]\theta\psi
       + \sqrt2\btheta\bar\psi\left[- 2\ii g\thth\btheta\bar\lambda^aT^a\right]\phi\notag\\
   &   + \ii\theta\Sm\btheta\left[\phi^*(2g\theta\Sm\btheta A^a_\mu T^a)\Pm\phi
        -\Pm\phi^*(2g\theta\Sm\btheta A^a_\mu T^a)\phi\right]\notag\\
   &   + 2\btheta\bar\psi\left[2g\theta\Sm\btheta A^a_\mu T^a\right]\theta\psi\notag\\
   & + \thth\bthth\left[
        F^*F+\frac14\phi^*\Psq\phi+\frac14\Psq\phi^*\phi
        -\frac12\Pm\phi^*\Pm\phi
        + \frac\ii2\Pm\bar\psi\bSm\psi
        - \frac\ii2\bar\psi\bSm\Pm\psi\right]\notag\\
\leadsto{}
   &  F^*F - D_\mu\phi^* D^\mu\phi - \ii\bar\psi\bSm D_\mu\psi\notag\\
   &  -gD^a(\phi^*T^a\phi) - \sqrt2\ii g\lambda^a(\phi^*T^a\psi)
       + \sqrt2\ii g\bar\lambda^a(\bar\psi T^a\phi)
\end{align}
\TODO{åvó Ç…ÇÊÇËïÑçÜÇ™àŸÇ»ÇÈÇ∆Ç¢Ç§â\ÅcÅc}
\begin{align}
 D_\mu\phi   &= (\Pm-\ii gA^{a\mu}T^a)\phi\\
 D_\mu\phi^* &= \Pm\phi^*+\ii gA^a_\mu(\phi^*T^a)\\
 D_\mu\psi   &= (\Pm-\ii gA^a_\mu T^a)\psi
\end{align}


\clearpage
\subsection{Minimal Supersymmetric Standard Model}
\subsubsection{Definitions}
\Paragraph{Gauge Group}
$\gSU(3)\s{color}\times\gSU(2)\s{weak}\times\gU(1)\s{Y}\quad(\times
{\gZ_2}_R\text{\ :\ $R$-parity})$
\paragraph{Fields}
\begin{center}\vspace{-1.7zw}
\begin{tabular}[t]{|c|ccc|c|c|}\hline
 Field      & $\gSU(3)$     & $\gSU(2)$ & $\gU(1)$ & $B$    & $L$  \\\hline
 $Q_i$      & $\vc 3$       & $\vc2$  & $ 1/6$ &  $1/3$ &      \\\hline
 $L_i$      &               & $\vc2$  & $-1/2$ &        &  $1$ \\\hline
 $\bar U_i$ & $\bar{\vc 3}$ &         & $-2/3$ & $-1/3$ &      \\\hline
 $\bar D_i$ & $\bar{\vc 3}$ &         & $ 1/3$ & $-1/3$ &      \\\hline
 $\bar E_i$ &               &         & $ 1  $ &        & $-1$ \\\hline
 $H\s u$    &               & $\vc2$  & $ 1/2$ &        &      \\\hline
 $H\s d$    &               & $\vc2$  & $-1/2$ &        &      \\\hline
\end{tabular}\hspace{2zw}
\begin{tabular}[t]{|c|ccc|}\hline
 Field      & $\gSU(3)$       & $\gSU(2)$ & $\gU(1)$ \\\hline
 $g$        & $\vc 8$       &         &        \\\hline
 $W$        &               & $\vc3$  &        \\\hline
 $B$        &               &         &        \\\hline
\end{tabular}
\end{center}

\def\Hu{{H\s u}}
\def\Hd{{H\s d}}
\def\bU{{\bar U}}
\def\bD{{\bar D}}
\def\bE{{\bar E}}

\paragraph{Superpotential}
\begin{align}
 W\s{RPC} &= \mu\Hu\Hd
           + {y\s u}_{ij} \Hu Q_i \bU_j
           + {y\s d}_{ij} \Hd Q_i \bD_j
           + {y\s e}_{ij} \Hd L_i \bE_j\\
 W\s{RPV} &= \mu_i\Hu L_i
           + {\lambda  }_{ijk} L_i L_j \bE_k
           + {\lambda' }_{ijk} L_i Q_j \bD_k
           + {\lambda''}_{ijk} \bU_i \bD_j \bD_k\\
&\hspace{13zw}
\text{(Here we define $\lambda_{ijk}=-\lambda_{jik}$ and $\lambda''_{ijk}=\lambda''_{ikj}$.)}\notag
\end{align}

\vspace{-2.5zw}
\subsubsection{Scalar Potential}
\paragraph{$F$-terms}
\begin{align}
-{{F_{\Hu}}^a}^*&= \epsilon^{ab}\left(
  \mu\Hd^b
+ {y\s u}_{ij} Q_i^{bx}\bU_j^x
+ \mu_i L_i^b
\right)\\
-{{F_{\Hd}}^a}^*&= \epsilon^{ab}\left(
- \mu\Hu^b
+ {y\s d}_{ij} Q_i^{bx}\bD_j^x
+ {y\s e}_{ij} L_i^{b} \bE_j
\right)\\
-{{F_{Q}}^{ax}_i}^*&= \epsilon^{ab}\left(
- {y\s u}_{ij} \Hu^{b} \bU_j^x
- {y\s d}_{ij} \Hd^{b} \bD_j^x
- {\lambda'}_{jik} L_i^b\bD_j^x
\right)\\
-{{F_{L}}^a_i}^*&= \epsilon^{ab}\left(
- \mu_i \Hu^b
- {y\s e}_{ij} \Hd^{b} \bE_j
+ 2\lambda_{ijk}L^b_j\bE_k
+ \lambda'_{ijk}Q_j^{bx}\bD_k^x
\right)\\
-{{F_{\bU}}^x_i}^*&=\left(
  \epsilon^{ab}{y\s u}_{ji}\Hu^a Q_j^{bx}
+ \epsilon^{xyz}\lambda''_{ijk}\bD_j^y\bD_k^z
\right)\\
-{{F_{\bD}}^x_i}^*&=\left(
  \epsilon^{ab}{y\s d}_{ji}\Hd^a Q_j^{bx}
+ \epsilon^{ab}{\lambda'}_{jki}L^a_j Q_k^{bx}
+ 2\epsilon^{yzx}\lambda''_{jki}\bU_j^y\bD_k^z
\right)\\
-{{F_{\bE}}_i}^*&=\left(
  \epsilon^{ab}{y\s e}_{ji}\Hd^a L_j^{b}
+ \epsilon^{ab}\lambda_{jki}L_j^aL_k^b
\right)
\end{align}
\vspace{-3zw}
\paragraph{$D$-terms}
\begin{align}
 {D_{g}}^\alpha &= -g_3\sum_{i=1}^3\left[
  \sum_{a=1,2}Q_i^{ax*}(T^\alpha)_{xy}Q_i^{ay}
- \bU_i^{x*}(T^\alpha)_{xy}\bU_i^{y}
- \bD_i^{x*}(T^\alpha)_{xy}\bD_i^{y}
\right]\\
%
 {D_{W}}^\alpha &= -g_2\left[
  \sum_{i=1}^3\sum_{x=1}^3 Q_i^{ax*}(T^\alpha)_{ab}Q_i^{by}
+ \sum_{i=1}^3 L_i^{a*}(T^\alpha)_{ab} L_i^{b}
+ \Hu^{a*}(T^\alpha)_{ab}\Hu^b
+ \Hd^{a*}(T^\alpha)_{ab}\Hd^b
\right]\\
%
 {D_{B}} &= -g_1\left[
  \frac16|  Q_i^{ax}|^2
- \frac12|  L_i^{a} |^2
- \frac23|\bU_i^{x} |^2
+ \frac13|\bD_i^{x} |^2
+        |\bE_i     |^2
+ \frac12|\Hu  ^{a} |^2
- \frac12|\Hd  ^{a} |^2
\right]
\end{align}

\paragraph{Full Scalar Potential}
\begin{equation}
 V = \sum|F_\bullet|^2+\frac12\sum|D_\bullet|^2
\end{equation}

%%% Local Variables:
%%% TeX-master: "CheatSheet.tex"
%%% End:
